Function for enciphering a message with an Enigma machine.

enigma.v
@@ -1,6 +1,8 @@
-Require Coq.Vectors.VectorDef.
-Require Coq.Vectors.Fin.
-Require Import Coq.Numbers.Natural.Peano.NPeano.
+Require Vectors.VectorDef.
+Require Vectors.Fin.
+Require Import Numbers.Natural.Peano.NPeano.
+Require Import Strings.String.
+Require Import Strings.Ascii.
 Require Import List.
 Require Import bijections.
 
@@ -510,6 +512,44 @@ Definition step_enigma (enigma : Enigma) : Enigma :=
 *)
 Definition press_key (enigma : Enigma) (a : Alpha) : (Alpha * Enigma) :=
   let enigma' := step_enigma enigma in (encipher enigma' a, enigma').
+
+
+Definition alpha_to_ascii (a : Alpha) : ascii :=
+  match Fin.to_nat a with
+  | exist _ a pf => ascii_of_nat ((nat_of_ascii "A") + a)
+  end.
+
+
+Definition ascii_to_alpha (a : ascii) : Alpha :=
+  match Compare_dec.lt_dec (nat_of_ascii a - nat_of_ascii "A") 26 with
+  | left pf_lt => Fin.of_nat_lt pf_lt
+  | right pf_ge => Fin.F1
+  end.
+
+
+Fixpoint string_to_alpha (str : string) : list Alpha :=
+  match str with
+  | EmptyString => nil
+  | String a str' => ascii_to_alpha a :: string_to_alpha str'
+  end.
+
+
+Definition alpha_to_string (alphas : list Alpha) : string :=
+  fold_left (fun str a => String (alpha_to_ascii a) str) (rev alphas) EmptyString.
+
+
+Example alpha_to_string_inverse_test :
+  alpha_to_string (string_to_alpha "HELLOWORLD") = "HELLOWORLD"%string.
+Proof. reflexivity. Qed.
+
+
+Fixpoint encipher_message (enigma : Enigma) (message : list Alpha) : (list Alpha) :=
+    match message with
+    | nil => nil
+    | a :: message' =>
+      let (o, enigma') := press_key enigma a in
+      o :: encipher_message enigma' message'
+    end.
 
 
 (* Need identical enigma machine to decipher (note: navy one was convertible...)
